Add a new module for working with logical relations

FunMaps.v
@@ -3,6 +3,7 @@ Require Import
   Here.Nomega
   Coq.Sets.Ensembles
   Here.TupleEnsembles
+  Here.LogicalRelations
   Coq.FSets.FMapList
   Coq.FSets.FMapFacts
   Coq.Structures.OrderedTypeEx.
@@ -12,7 +13,7 @@ Module FunMaps (O : OrderedType).
 Module E := FMapExt(O).
 Include E.
 
-Definition SetMap_AbsR
+Definition Map_AbsR
            (A B : Type) (R  : A -> B -> Prop)
            (or : Ensemble (M.key * A))
            (nr : M.t B) : Prop :=
@@ -24,20 +25,10 @@ Definition SetMap_AbsR
        M.find addr nr = Some cblk
          -> (exists blk, Lookup addr blk or /\ R blk cblk)).
 
-Ltac reduction :=
+Ltac reduce_context :=
   try repeat teardown; subst;
   match goal with
-  | [ _ : ?T -> ?U -> Prop,
-      H1 : SetMap_AbsR _ _ _,
-      H2 : Lookup ?A ?D ?K |- exists _ : ?U, _ ] =>
-    let HA := fresh "HA" in
-    destruct (H1 A) as [HA _];
-    let HC := fresh "HC" in
-    let HD := fresh "HC" in
-    let cblk := fresh "cblk" in
-    destruct (HA _ H2) as [cblk [HC HD]]; clear HA H2;
-    exists cblk; split; trivial
-  | [ H1 : SetMap_AbsR _ _ _,
+  | [ H1 : Map_AbsR _ _ _,
       H2 : Lookup ?A ?D ?K |- _ ] =>
     let HA := fresh "HA" in
     let HB := fresh "HB" in
@@ -46,17 +37,7 @@ Ltac reduction :=
     let HD := fresh "HD" in
     let cblk := fresh "cblk" in
     destruct (HA _ H2) as [cblk [HC HD]]; clear HA HB H2
-  | [ _ : ?T -> ?U -> Prop,
-      H1 : SetMap_AbsR _ _ _,
-      H2 : M.find ?A ?K = Some ?D |- exists _ : ?T, _ ] =>
-    let HB := fresh "HB" in
-    destruct (H1 A) as [_ HB];
-    let HC := fresh "HC" in
-    let HD := fresh "HD" in
-    let blk := fresh "blk" in
-    destruct (HB _ H2) as [blk [HC HD]]; clear HB H2;
-    exists blk; split; trivial
-  | [ H1 : SetMap_AbsR _ _ _,
+  | [ H1 : Map_AbsR _ _ _,
       H2 : M.find ?A ?K = Some ?D |- _ ] =>
     let HA := fresh "HA" in
     let HB := fresh "HB" in
@@ -67,193 +48,446 @@ Ltac reduction :=
     destruct (HB _ H2) as [blk [HC HD]]; clear HA HB H2
   end.
 
+Ltac reduction :=
+  try repeat teardown; subst;
+  match goal with
+  | [ _ : ?T -> ?U -> Prop,
+      H1 : Map_AbsR _ _ _,
+      H2 : Lookup ?A ?D ?K |- exists _ : ?U, _ ] =>
+    let HA := fresh "HA" in
+    destruct (H1 A) as [HA _];
+    let HC := fresh "HC" in
+    let HD := fresh "HC" in
+    let cblk := fresh "cblk" in
+    destruct (HA _ H2) as [cblk [HC HD]]; clear HA H2;
+    exists cblk; split; trivial
+  | [ H1 : Map_AbsR _ _ _,
+      H2 : Lookup ?A ?D ?K |- _ ] =>
+    let HA := fresh "HA" in
+    let HB := fresh "HB" in
+    destruct (H1 A) as [HA HB];
+    let HC := fresh "HC" in
+    let HD := fresh "HD" in
+    let cblk := fresh "cblk" in
+    destruct (HA _ H2) as [cblk [HC HD]]; clear HA HB H2
+  | [ _ : ?T -> ?U -> Prop,
+      H1 : Map_AbsR _ _ _,
+      H2 : M.find ?A ?K = Some ?D |- exists _ : ?T, _ ] =>
+    let HB := fresh "HB" in
+    destruct (H1 A) as [_ HB];
+    let HC := fresh "HC" in
+    let HD := fresh "HD" in
+    let blk := fresh "blk" in
+    destruct (HB _ H2) as [blk [HC HD]]; clear HB H2;
+    exists blk; split; trivial
+  | [ H1 : Map_AbsR _ _ _,
+      H2 : M.find ?A ?K = Some ?D |- _ ] =>
+    let HA := fresh "HA" in
+    let HB := fresh "HB" in
+    destruct (H1 A) as [HA HB];
+    let HC := fresh "HC" in
+    let HD := fresh "HD" in
+    let blk := fresh "blk" in
+    destruct (HB _ H2) as [blk [HC HD]]; clear HA HB H2
+  end.
+
+Ltac simplify_maps :=
+  match goal with
+  | [ H : M.find (elt:=?T) ?A (M.add ?K ?E ?M) = Some ?B |- _ ] =>
+    apply F.find_mapsto_iff, F.add_mapsto_iff in H;
+    let H1 := fresh "H1" in
+    let H2 := fresh "H2" in
+    let H3 := fresh "H3" in
+    let H4 := fresh "H4" in
+    destruct H as [[H1 H2]|[H3 H4]];
+    [subst|apply F.find_mapsto_iff in H4]
+  | [ H : M.find (elt:=?T) ?A (M.remove ?KE ?M) = Some ?B |- _ ] =>
+    apply F.find_mapsto_iff, F.remove_mapsto_iff in H;
+    let H1 := fresh "H1" in
+    let H2 := fresh "H2" in
+    destruct H as [H1 H2];
+    apply F.find_mapsto_iff in H2
+  | [ H : M.find (elt:=?T) ?A (M.map ?F ?M) = Some ?B |- _ ] =>
+    apply F.find_mapsto_iff, F.map_mapsto_iff in H;
+    let cblk := fresh "cblk" in
+    let H1 := fresh "H1" in
+    let H2 := fresh "H2" in
+    destruct H as [cblk [H1 H2]];
+    apply F.find_mapsto_iff in H2
+  | [ H : M.find (elt:=?T) ?A (P.filter ?F ?M) = Some ?B |- _ ] =>
+    apply F.find_mapsto_iff, P.filter_iff in H;
+    [let H1 := fresh "H1" in
+     let H2 := fresh "H2" in
+     destruct H as [H1 H2];
+     apply F.find_mapsto_iff in H1|]
+  | [ H : M.find (elt:=?T) ?A (M.mapi ?F ?M) = Some ?B |- _ ] =>
+    rewrite F.mapi_o, <- F.map_o in H
+  | [ H : M.find (elt:=?T) ?A (M.empty ?U) = Some ?B |- _ ] =>
+    apply F.find_mapsto_iff, F.empty_mapsto_iff in H;
+    contradiction
+  | [ H1 : M.find (elt:=?T) ?A ?M = Some ?B,
+      H2 : M.Empty (elt:=?T) ?M |- _ ] =>
+    apply P.elements_Empty in H2;
+    rewrite F.elements_o in H1;
+    rewrite H2 in H1;
+    inversion H1
+  end.
+
+Corollary Map_AbsR_A {A B} (R : A -> B -> Prop)
+          (or : Ensemble (M.key * A))
+          (nr : M.t B) :
+  Map_AbsR R or nr ->
+  forall addr blk,
+    Lookup addr blk or ->
+      exists cblk, M.find addr nr = Some cblk /\ R blk cblk.
+Proof. intros; reduction. Qed.
+
+Corollary Map_AbsR_B {A B} (R : A -> B -> Prop)
+          (or : Ensemble (M.key * A))
+          (nr : M.t B) :
+  Map_AbsR R or nr ->
+  forall addr cblk,
+    M.find addr nr = Some cblk ->
+      exists blk, Lookup addr blk or /\ R blk cblk.
+Proof. intros; reduction. Qed.
+
+Lemma Oeq_neq_sym : forall x y, ~ O.eq x y -> ~ O.eq y x.
+Proof.
+  intros.
+  unfold not; intros.
+  rewrite H0 in H.
+  contradiction H.
+  apply O.eq_refl.
+Qed.
+
 Section FunMaps_AbsR.
 
 Variables A B : Type.
-Variable R  : A -> B -> Prop.
-Variable or : Ensemble (M.key * A).
-Variable nr : M.t B.
-Variable AbsR : SetMap_AbsR R or nr.
+Variable R : (A -> B -> Prop).
 
-Lemma Empty_SetMap_AbsR : SetMap_AbsR R Empty (M.empty B).
-Proof.
-  split; intros.
-    inversion H.
-  apply F.find_mapsto_iff, F.empty_mapsto_iff in H.
-  contradiction.
-Qed.
+Hypothesis Oeq_eq : forall a b, O.eq a b <-> a = b.
+Hypothesis Oeq_neq : forall a b, ~ O.eq a b <-> a <> b.
 
-Corollary SetMap_AbsR_prj1 : forall (addr : M.key) (blk : A) cblk,
-  Lookup addr blk or
-    -> (forall a b c, R a b -> R a c -> b = c)
-    -> R blk cblk
-    -> M.find (elt:=B) addr nr = Some cblk.
-Proof. intros; reduction; rewrite (H0 _ _ _ H1 HD); assumption. Qed.
+Ltac equalities :=
+  repeat
+    match goal with
+    | [ H : O.eq ?X ?Y |- _ ] =>
+      apply Oeq_eq in H; subst
+    | [ H : ?X <> ?X |- _ ] =>
+      contradiction H; reflexivity
+    | [ H : ?X <> ?Y |- _ ] =>
+      apply Oeq_neq in H; subst
+    | [ |- ?X <> ?Y ] =>
+      unfold not; intros; subst
+    | [ |- ~ O.eq ?X ?Y ] =>
+      let H := fresh "H" in
+      unfold not; intro H;
+      apply Oeq_eq in H; subst
+    | [ |- O.eq ?X ?Y -> False ] =>
+      let H := fresh "H" in
+      unfold not; intro H;
+      apply Oeq_eq in H; subst
+    | [ |- O.eq ?X ?X ] =>
+      apply O.eq_refl
+    | [ H : ~ O.eq ?X ?X |- _ ] =>
+      contradiction H; apply O.eq_refl
+    | [ H : O.eq ?X ?X -> False |- _ ] =>
+      contradiction H; apply O.eq_refl
+    | [ |- ?X = ?X ] =>
+      reflexivity
+    end.
 
-Corollary SetMap_AbsR_prj1_ex : forall (addr : M.key) (blk : A),
-  Lookup addr blk or
-    -> exists cblk : B,
-         M.find (elt:=B) addr nr = Some cblk /\ R blk cblk.
-Proof. intros; reduction. Qed.
-
-Corollary SetMap_AbsR_prj2_ex : forall (addr : M.key) (cblk : B),
-  M.find (elt:=B) addr nr = Some cblk
-    -> exists blk : A, Lookup addr blk or /\ R blk cblk.
-Proof. intros. reduction. Qed.
-
-Hypothesis Oeq_eq : forall a b, O.eq a b -> a = b.
-
-Lemma Update_SetMap_AbsR : forall k v v',
-  R v v' -> SetMap_AbsR R (Update k v or) (M.add k v' nr).
-Proof.
-  split; intros.
-  - repeat teardown; subst.
-    + exists v'; split; trivial.
-      apply F.find_mapsto_iff, F.add_mapsto_iff.
-      left; auto.
-    + reduction.
-      apply F.find_mapsto_iff in HC.
-      apply F.find_mapsto_iff, F.add_mapsto_iff.
-      right; split; auto.
-  - apply F.find_mapsto_iff, F.add_mapsto_iff in H0.
-    destruct H0, H0; subst.
-      exists v; split; trivial.
-      apply Oeq_eq in H0; subst.
-      right; constructor.
-    apply F.find_mapsto_iff in H1.
-    reduction.
-    left; constructor; auto.
-    unfold Ensembles.In; simpl.
-    unfold not; intros.
-    subst; auto.
-Qed.
-
-Lemma Remove_SetMap_AbsR : forall k,
-  SetMap_AbsR R (Remove k or) (M.remove k nr).
-Proof.
-  split; intros.
-    reduction.
-    apply F.find_mapsto_iff, F.remove_mapsto_iff.
-    split; auto.
-    apply F.find_mapsto_iff.
-    assumption.
-  apply F.find_mapsto_iff, F.remove_mapsto_iff in H.
-  destruct H.
-  apply F.find_mapsto_iff in H0.
-  reduction.
-  constructor; trivial.
-  unfold Ensembles.In; simpl.
-  unfold not; intros.
-  subst; auto.
-Qed.
-
-Lemma Map_SetMap_AbsR : forall f f',
-  (forall i a b, R a b -> R (f i a) (f' i b))
-    -> SetMap_AbsR R (Map f or) (M.mapi f' nr).
-Proof.
-  split; intros.
-    repeat teardown; subst.
-    destruct (AbsR addr); clear H2.
-    destruct (H0 _ H1) as [cblk [? ?]]; clear H0 H1.
-    exists (f' addr cblk).
-    apply F.find_mapsto_iff in H2.
-    split.
-      rewrite F.mapi_o, <- F.map_o.
-        apply F.find_mapsto_iff.
-        apply F.map_mapsto_iff.
-        exists cblk; tauto.
-      intros.
-      apply Oeq_eq in H0.
-      subst; reflexivity.
-    apply H; trivial.
-  rewrite F.mapi_o, <- F.map_o in H0.
-    apply F.find_mapsto_iff in H0.
-    apply F.map_mapsto_iff in H0.
-    repeat teardown; subst.
-    apply F.find_mapsto_iff in H1.
-    destruct (AbsR addr); clear H0.
-    destruct (H2 _ H1) as [blk [? ?]]; clear H1 H2.
-    exists (f addr blk).
-    split.
-      teardown.
-    apply H; trivial.
-  intros.
-  apply Oeq_eq in H1.
-  subst; reflexivity.
-Qed.
-
-Lemma Proper_Oeq_negb : forall f,
+Corollary Proper_Oeq_negb : forall B f,
   Proper (O.eq ==> eq ==> eq) f ->
   Proper (O.eq ==> eq ==> eq) (fun (k : M.key) (e : B) => negb (f k e)).
-Proof.
-  intros.
-  intros x y H1 x' y' H2. subst.
-  apply Oeq_eq in H1; subst.
-  reflexivity.
-Qed.
+Proof. intros ?????????; equalities. Qed.
 
-Lemma Single_SetMap_AbsR : forall base blk cblk,
-  R blk cblk -> SetMap_AbsR R (Single base blk) (singleton base cblk).
-Proof.
-  intros.
-  intro addr.
+Export LogicalRelationNotations.
+
+Open Scope lsignature_scope.
+
+Program Instance Empty_Map_AbsR : Empty [R Map_AbsR R] (M.empty _).
+Obligation 1. split; intros; [ inversion H | simplify_maps ]. Qed.
+
+Program Instance Single_Map_AbsR :
+  (@Single _ _) [R O.eq ===> R ===> Map_AbsR R] singleton.
+Obligation 1.
+  intros ??????.
   split; intros;
-  [exists cblk|exists blk].
+  [exists y0|exists x0];
+  equalities.
     repeat teardown; subst.
     split; trivial.
-    unfold P.uncurry.
+    unfold P.uncurry; simpl.
     rewrite F.elements_o; simpl.
-    rewrite eqb_refl.
-    reflexivity.
-  rewrite F.elements_o in H0; simpl in H0.
-  unfold F.eqb in H0.
-  destruct (O.eq_dec addr base).
-    inversion H0.
-    apply Oeq_eq in e.
-    subst.
+    rewrite eqb_refl; trivial.
+  rewrite F.elements_o in H1; simpl in H1.
+  unfold F.eqb in H1.
+  destruct (O.eq_dec addr y).
+    inversion H1.
+    equalities.
     split; trivial.
     apply Lookup_Single.
   discriminate.
 Qed.
 
-End FunMaps_AbsR.
-
-Lemma Same_set_SetMap_AbsR : forall A B (R : A -> B -> Prop) a b r,
-  Same a b
-    -> SetMap_AbsR R a r
-    -> SetMap_AbsR R b r.
-Proof.
-  intros.
-  intros addr.
-  destruct (H0 addr).
-  split; intros.
-    apply H in H3.
-    destruct (H1 _ H3) as [cblk [? ?]].
-    exists cblk.
-    intuition.
-  destruct (H2 _ H3) as [blk [? ?]].
-  exists blk.
-  split; trivial.
-  apply H; trivial.
+Program Instance Lookup_Map_AbsR
+        `{LogicalImpl _ _ R eq} `{LogicalDep _ _ R eq} :
+  (@Lookup _ _) [R O.eq ===> R ===> Map_AbsR R ===> iff]
+  (fun k e m => M.find k m = Some e).
+Obligation 1.
+  intros ?????????.
+  split; intros; equalities; reduction;
+  [ pose proof (forward_impl _ _ _ H2 HD)
+  | pose proof (reverse_impl _ _ _ H2 HD) ];
+  subst; assumption.
 Qed.
 
-Lemma Equal_SetMap_AbsR : forall A B (R : A -> B -> Prop) a b r,
-  M.Equal a b
-    -> SetMap_AbsR R r a
-    -> SetMap_AbsR R r b.
+Program Instance Lookup_MapsTo_Map_AbsR
+        `{LogicalImpl _ _ R eq} `{LogicalDep _ _ R eq} :
+  (@Lookup _ _) [R O.eq ===> R ===> Map_AbsR R ===> iff]
+  (fun k e m => M.find k m = Some e).
+Obligation 1.
+  intros ?????????.
+  split; intros; equalities; reduction;
+  [ pose proof (forward_impl _ _ _ H2 HD)
+  | pose proof (reverse_impl _ _ _ H2 HD) ];
+  subst; assumption.
+Qed.
+
+Program Instance Same_Map_AbsR
+        `{LogicalImpl _ _ R eq} `{LogicalDep _ _ R eq} :
+  (@Same _ _) [R Map_AbsR R ===> Map_AbsR R ===> iff] M.Equal.
+Obligation 1.
+  intros ??????.
+  split; intros.
+    apply F.Equal_mapsto_iff; split; intros.
+      apply F.find_mapsto_iff in H4;
+      apply F.find_mapsto_iff.
+      reduce_context.
+      rewrite H3 in HC.
+      reduction.
+      pose proof (forward_impl _ _ _ HD HD0);
+      subst; assumption.
+    apply F.find_mapsto_iff in H4;
+    apply F.find_mapsto_iff.
+    reduction.
+    apply H3 in HC.
+    reduction.
+    pose proof (forward_impl _ _ _ HD HD0);
+    subst; assumption.
+  split; intros.
+    reduction.
+    rewrite H3 in HC.
+    reduction.
+    pose proof (reverse_impl _ _ _ HD HD0);
+    subst; assumption.
+  reduction.
+  rewrite <- H3 in HC.
+  reduction.
+  pose proof (reverse_impl _ _ _ HD HD0);
+  subst; assumption.
+Qed.
+
+Program Instance Member_Map_AbsR :
+  (@Member _ _) [R O.eq ===> Map_AbsR R ===> boolR] (@M.mem _).
+Obligation 1.
+  unfold Member; intros ??????.
+  rewrite F.mem_find_b.
+  split; intros; equalities.
+    reduction.
+    rewrite HC.
+    reflexivity.
+  destruct (M.find (elt:=B) y y0) eqn:Heqe.
+    reduction.
+    exists blk.
+    assumption.
+  discriminate.
+Qed.
+
+Lemma has_Some : forall A B (a : option A) (b : B),
+  a <> None -> exists b, a = Some b.
 Proof.
   intros.
-  intros addr.
-  destruct (H0 addr).
-  split; intros.
-    destruct (H1 _ H3) as [cblk [? ?]].
-    exists cblk.
-    split; trivial.
-    rewrite <- H; trivial.
-  rewrite <- H in H3.
-  destruct (H2 _ H3) as [blk [? ?]].
+  destruct a.
+    exists a; reflexivity.
+  contradiction H.
+  reflexivity.
+Qed.
+
+Program Instance Member_In_Map_AbsR :
+  (@Member _ _) [R O.eq ===> Map_AbsR R ===> iff] (@M.In _).
+Obligation 1.
+  unfold Member; intros ??????.
+  split; intros; equalities.
+    destruct H1.
+    reduction.
+    apply F.in_find_iff.
+    rewrite HC.
+    apply Common.Some_ne_None.
+  apply F.in_find_iff in H1.
+  eapply has_Some in H1; eauto.
+  destruct H1.
+  reduction.
   exists blk.
-  intuition.
+  assumption.
+Qed.
+
+(* Insert *)
+
+Program Instance Remove_Map_AbsR :
+  (@Remove _ _) [R O.eq ===> Map_AbsR R ===> Map_AbsR R] (@M.remove _).
+Obligation 1.
+  intros ??????.
+  split; intros.
+  - reduction; equalities.
+    apply Oeq_neq_sym in H1.
+    rewrite F.remove_neq_o; trivial.
+  - simplify_maps; reduction.
+    teardown; equalities.
+Qed.
+
+Program Instance Update_Map_AbsR :
+  (@Update _ _) [R O.eq ===> R ===> Map_AbsR R ===> Map_AbsR R] (@M.add _).
+Obligation 1.
+  intros ?????????.
+  split; intros; repeat teardown; subst.
+  - exists y0; intuition.
+    apply F.add_eq_o; symmetry; assumption.
+  - reduction; equalities.
+    apply Oeq_neq_sym in H2.
+    rewrite F.add_neq_o; trivial.
+  - simplify_maps.
+      exists x0.
+      intuition; equalities.
+      right; constructor.
+    reduction; teardown.
+    right; constructor;
+    equalities; assumption.
+Qed.
+
+(* Move *)
+
+Program Instance Map_Map_AbsR :
+  (@Map _ _) [R (O.eq ===> R ===> R) ===> Map_AbsR R ===> Map_AbsR R]
+  (@M.mapi _ _).
+Obligation 1.
+  intros ??????.
+  split; intros.
+  - teardown.
+    do 2 destruct H1.
+    reduce_context.
+    exists (y addr cblk).
+    split.
+      rewrite F.mapi_o, <- F.map_o.
+        apply F.find_mapsto_iff, F.map_mapsto_iff.
+        exists cblk; intuition.
+        apply F.find_mapsto_iff; assumption.
+      intros; equalities.
+    apply H; trivial.
+  - simplify_maps.
+      simplify_maps.
+      reduce_context.
+      exists (x addr blk).
+      split.
+        teardown.
+      apply H; trivial.
+    intros; equalities.
+Qed.
+
+Program Instance Filter_Map_AbsR :
+  (@Filter _ _) [R (O.eq ===> R ===> boolR) ===> Map_AbsR R ===> Map_AbsR R]
+  (@P.filter _).
+Obligation 1.
+  intros ??????.
+  split; intros.
+    reduction.
+    apply F.find_mapsto_iff, P.filter_iff.
+      intros ??????; subst; equalities.
+    split.
+      apply F.find_mapsto_iff; trivial.
+    eapply H in H1; eauto.
+  simplify_maps.
+  reduction.
+  eexists; simpl; trivial.
+    eapply H in H3; eauto.
+  intros ??????; subst; equalities.
+Qed.
+
+(* Define *)
+(* Modify *)
+(* Overlay *)
+
+Program Instance All_Map_AbsR :
+  (@All _ _) [R (O.eq ===> R ===> boolR) ===> Map_AbsR R ===> boolR]
+  (@P.for_all _).
+Obligation 1.
+  intros ??????.
+  split; intros;
+  unfold All, P.for_all in *.
+    apply P.fold_rec_bis; intros; trivial; subst.
+    apply F.find_mapsto_iff in H2.
+    reduction.
+    apply H1 in HC.
+    eapply H in HC; eauto.
+    rewrite HC.
+    reflexivity.
+  intros.
+  reduction.
+  eapply H; eauto.
+  revert H1.
+  revert HC.
+  apply P.fold_rec; intros; subst; intuition.
+    simplify_maps.
+  rewrite H3 in HC.
+  simplify_maps.
+    equalities.
+    destruct (y a cblk) eqn:Heqe; intuition.
+  destruct (y k e) eqn:Heqe; intuition.
+Qed.
+
+Program Instance Any_Map_AbsR :
+  (@Any _ _) [R (O.eq ===> R ===> boolR) ===> Map_AbsR R ===> boolR]
+  (@P.exists_ _).
+Obligation 1.
+  intros ??????.
+  split; intros;
+  unfold Any in *.
+    apply P.exists_iff.
+      intros ??????; subst; equalities.
+    do 3 destruct H1.
+    reduction.
+    exists (x1, cblk).
+    split; simpl.
+      apply F.find_mapsto_iff; assumption.
+    eapply H; eauto.
+  apply P.exists_iff in H1.
+    do 2 destruct H1.
+    apply F.find_mapsto_iff in H1.
+    reduction.
+    exists k.
+    exists blk.
+    split; trivial.
+    eapply H; eauto.
+  intros ??????; subst; equalities.
+Qed.
+
+End FunMaps_AbsR.
+
+Program Instance Same_set_Map_AbsR : forall A B (R : A -> B -> Prop),
+  Proper (eq ==> @Same _ _ ==> @M.Equal _ ==> iff) (@Map_AbsR A B).
+Obligation 1.
+  intros ?????????.
+  split; intros;
+  split; intros; subst.
+  - apply H0 in H3; reduction.
+    rewrite <- H1; assumption.
+  - rewrite <- H1 in H3; reduction.
+    apply H0 in HC; assumption.
+  - apply H0 in H3; reduction.
+    rewrite H1; assumption.
+  - rewrite H1 in H3; reduction.
+    apply H0; assumption.
 Qed.
 
 End FunMaps.
