LogicalRelations.v
@@ -1,0 +1,65 @@
+Require Export
+  Coq.Classes.Morphisms
+  Coq.Classes.RelationClasses
+  Relation_Definitions.
+
+Class LogicalRelation {A B} (R : A -> B -> Prop) (m : A) (m' : B) := {
+  logical_prf : R m m'
+}.
+
+Class LogicalImpl {A B} (R : A -> B -> Prop)
+      (eqv : relation B) (m : A) (m' : B) := {
+  impl_logical_rel :> LogicalRelation R m m';
+  forward_impl : forall a b c, R a b -> R a c -> eqv b c
+}.
+
+Class LogicalDep {A B} (R : A -> B -> Prop)
+      (dep : relation A) (m : A) (m' : B) := {
+  dep_logical_rel :> LogicalRelation R m m';
+  reverse_impl : forall a b c, R a c -> R b c -> dep a b
+}.
+
+Definition related_hetero
+           (A B : Type)
+           (C : A -> Type) (D : B -> Type)
+           (R : A -> B -> Prop)
+           (R' : forall (x : A) (y : B), C x -> D y -> Prop) :
+  (forall x : A, C x) -> (forall x : B, D x) -> Prop :=
+  fun f g => forall x y, R x y -> R' x y (f x) (g y).
+
+Definition related {A B C D} (R : A -> B -> Prop)
+           (R' : C -> D -> Prop) : (A -> C) -> (B -> D) -> Prop :=
+  Eval compute in @related_hetero A B (fun _ => C) (fun _ => D) R (fun _ _ => R').
+
+(** Notations reminiscent of the old syntax for declaring morphisms. *)
+Delimit Scope lsignature_scope with lsignature.
+
+Module LogicalRelationNotations.
+
+  Notation " R +++> R' " := (@related _ _ _ _ (R%lsignature) (R'%lsignature))
+    (right associativity, at level 55) : lsignature_scope.
+
+  Notation " R ===> R' " := (@related _ _ _ _ (R%lsignature) (R'%lsignature))
+    (right associativity, at level 55) : lsignature_scope.
+
+  Notation " R ---> R' " := (@related _ _ _ _ (Basics.flip (R%lsignature)) (R'%lsignature))
+    (right associativity, at level 55) : lsignature_scope.
+
+  Notation "f [R  rel ] f'" := (LogicalRelation rel f f')
+    (right associativity, at level 55) : lsignature_scope.
+
+End LogicalRelationNotations.
+
+Arguments LogicalRelation {A}%type {B}%type R%lsignature m m'.
+Arguments related {A B C D}%type (R R')%lsignature _ _.
+
+Export LogicalRelationNotations.
+
+Local Open Scope lsignature_scope.
+
+Arguments LogicalRelation : default implicits.
+
+Program Instance Equality_LogicalRelation : forall A (x : A),
+  x [R eq] x.
+
+Definition boolR (P : Prop) (b : bool) : Prop := P <-> b = true.
