TupleEnsemblesFinite.v
@@ -34,47 +34,166 @@ Qed.
 
 Lemma Conjunction_preserves_finite {U} :
   forall A:Ensemble U,
-    Finite U A -> forall X:Ensemble U, Finite U (fun x : U => In U X x /\ In U A x).
+    Finite U A -> forall X:Ensemble U,
+      Finite U (fun x : U => In U X x /\ In U A x) <-> Finite U (In U A).
 Proof.
-  intros A' H' X; apply Finite_downward_closed with A'; auto with sets.
+  intros A' H' X.
+  split; intros.
+    apply Finite_downward_closed with A'; auto with sets.
+  apply Finite_downward_closed with A'; auto with sets.
   intros ? H0; inversion H0; assumption.
 Qed.
 
-Lemma Remove_Finite : forall a `(_ : Finite _ r), Finite _ (@Remove A B a r).
+Lemma Conjunction_preserves_finite_2 {U} :
+  forall A:Ensemble U,
+    Finite U A -> forall X:Ensemble U,
+      Finite U (fun x : U => In U A x /\ In U X x) -> Finite U (In U A).
 Proof.
-  unfold Remove; simpl; intros.
-  apply Setminus_preserves_finite; assumption.
+  intros A' H' X H.
+  apply Finite_downward_closed with A'; auto with sets.
 Qed.
 
-Lemma Update_Finite : forall a b `(_ : Finite _ r), Finite _ (@Update A B a b r).
+Lemma Exists_preserves_finite_conj {U V} :
+  forall (f : U * V -> V -> U * V) (X : Ensemble (U * V)) z,
+    Finite (U * V) (fun x : U * V =>
+                      exists b : V, In (U * V) X (f x b)) ->
+    Finite (U * V) (fun x : U * V =>
+                      exists b : V, In (U * V) X (f x b) /\ z x b).
 Proof.
-  unfold Remove; simpl; intros.
-  apply Add_preserves_Finite, Setminus_preserves_finite; assumption.
+  intros.
+  eapply Finite_downward_closed; eauto with sets.
+  intros ? H0; inversion H0; intuition; clear H0.
+  exists x0.
+  assumption.
+Qed.
+
+Lemma Exists_finite_forall {U V} :
+  forall (X:Ensemble (U * V)),
+    Finite (U * V) X ->
+    Finite (U * V) (fun x : U * V => exists b : V, In (U * V) X (fst x, b)).
+Proof.
+  intros.
+  inversion H.
+    admit.
+  eapply Finite_downward_closed; eauto with sets.
+  intros ? H3; inversion H3; intuition; clear H3.
+  rewrite H2 in H4.
+Abort.
+
+Lemma Exists_preserves_finite {U V} :
+  forall (X:Ensemble (U * V)),
+    Finite (U * V) X ->
+    Finite (U * V) (fun x : U * V => exists b : V, In (U * V) X (fst x, b)).
+Proof.
+  intros.
+(*
+  apply ex_Included; intros.
+  pose proof (ex_Included (U * V) V (fun b x => (fst x, b)) X).
+  intros ? H0; inversion H0; intuition; clear H0.
+    inversion H.
+  inversion IHFinite.
+    admit.
+  eapply Finite_downward_closed; eauto with sets.
+  intros ? H4; inversion H4; intuition; clear H4.
+  inversion H5; subst; clear H5.
+    admit.
+  inversion H4; subst; clear H4.
+    contradiction.
+  inversion H2; subst; clear H2.
+    admit.
+  inversion H1; subst; clear H1.
+    rewrite (Non_disjoint_union U X x); auto with sets.
+  unfold Ensembles.In.
+  inversion H2; subst; clear H2.
+    exists x1.
+    assumption.
+  assumption.
+*)
+Abort.
+
+Lemma Remove_Finite : forall a `(_ : Finite _ r), Finite _ (@Remove A B a r).
+Proof. intros; apply Setminus_preserves_finite; assumption. Qed.
+
+Lemma Update_Finite : forall a b `(_ : Finite _ r),
+  Finite _ (@Update A B a b r).
+Proof.
+  intros; apply Add_preserves_Finite, Setminus_preserves_finite; assumption.
 Qed.
 
 Lemma Move_Finite : forall a a' `(_ : Finite _ r), Finite _ (@Move A B a a' r).
 Proof.
+  unfold Move; intros.
+  eapply Finite_downward_closed; eauto with sets.
+  intros ? H0.
+  unfold Ensembles.In in H0.
+  destruct H0.
+    destruct H; subst.
+    admit.
+  destruct H.
+  teardown.
+  destruct H0.
+  unfold Lookup in H1.
+  rewrite <- surjective_pairing in H1.
+  assumption.
 Admitted.
 
 Lemma Filter_Finite : forall P `(_ : Finite _ r), Finite _ (@Filter A B P r).
 Proof.
-Admitted.
+  unfold Filter; intros.
+  eapply Finite_downward_closed; eauto with sets.
+  intros ? H0; inversion H0; clear H0.
+  unfold Lookup in H.
+  rewrite <- surjective_pairing in H.
+  assumption.
+Qed.
 
 Lemma Map_Finite : forall f `(_ : Finite _ r), Finite _ (@Map A B f r).
 Proof.
+  unfold Map, Lookup; intros.
+  apply Exists_preserves_finite_conj.
+  eapply Finite_downward_closed; eauto with sets.
+  intros ? H0.
+  destruct H0.
+  destruct x; simpl in *.
+  induction Finite0.
+    admit.
 Admitted.
 
 Lemma Modify_Finite : forall a f `(_ : Finite _ r), Finite _ (@Modify A B a f r).
 Proof.
+  unfold Modify; intros.
+  eapply Finite_downward_closed; eauto with sets.
+  intros ? H0.
+  unfold Ensembles.In in H0.
+  destruct H0, H; subst.
+  destruct H0, H; subst.
+  inversion H0; subst; clear H0.
+  unfold Lookup in H.
+  admit.
 Admitted.
 
 Lemma Define_Finite : forall P b `(_ : Finite _ r), Finite _ (@Define A B P b r).
 Proof.
+  unfold Define; intros.
+  eapply Finite_downward_closed; eauto with sets.
+  intros ? H0.
+  unfold Ensembles.In in H0.
+  admit.
 Admitted.
 
 Lemma Overlay_Finite : forall P `(_ : Finite _ r) `(_ : Finite _ r'),
   Finite _ (@Overlay A B P r r').
 Proof.
+  unfold Overlay; intros.
+  eapply Finite_downward_closed; eauto with sets.
+  intros ? H0.
+  unfold Ensembles.In in H0.
+  specialize (H0 (fst x)).
+  destruct H0, H; subst.
+    unfold Lookup in H0.
+    rewrite <- surjective_pairing in H0.
+    assumption.
+  admit.
 Admitted.
 
 End TupleEnsembleFinite.
